[ec kemdem] improve notations and avoid nerdisms in proofs

kemdem/EasyCrypt/KEMDEM.ec
@@ -1,31 +1,36 @@
-(* As specified in Boneh and Shoup's "Graduate Course in Applied Cryptography"
-     https://toc.cryptobook.us/
-   (Exercise 11.9 of version 0.6.)
-*)
+(*^
+  As specified in Boneh and Shoup's "Graduate Course in Applied Cryptography"
+  https://toc.cryptobook.us/
+  (Exercise 11.9 of version 0.6.)
+^*)
 require import AllCore Distr.
 
-(** A more mature proof would rely on libraries of definitions-generic
-    definitions have a lot more parameters than what we'd like to
-    expose a tutorial reader to.
+(*^
+  A more mature proof would rely on libraries of definitions.
+  Generic definitions have a lot more parameters than what
+  we'd like to expose a tutorial reader to.
 
-    Instead, we inline (and specialise) the definitions we care about.
-**)
+  Instead, we inline (and specialize) the definitions we care about.
+^*)
 
-(* Given sets of public keys, secret keys, plaintexts, DEM keys, KEM
-   ciphertexts and DEM ciphertexts ... *)
-type pkey, skey, pt, key, kct, dct.
+(*
+  Given sets of public keys, secret keys, symmetric (DEM) keys,
+  KEM ciphertexts, plaintexts, and DEM ciphertexts ...
+*)
+type pkey, skey, key, kct, pt, dct.
 
-(* ... and the uniform distribution over the DEM key space *)
+(* ... and the uniform distribution over the set of symmetric (DEM) keys *)
 op [lossless full uniform] dkey : key distr.
 
 
-(** A KEM is a triple of (potentially probabilistic and stateful)
-    algorithms:
+(**
+  A KEM is a triple of (potentially probabilistic and stateful)
+  algorithms:
 **)
 module type KEM = {
   proc keygen(): pkey * skey
-  proc enc(pk : pkey): key * kct
-  proc dec(sk : skey, k : kct): key option
+  proc encaps(pk : pkey): key * kct
+  proc decaps(sk : skey, k : kct): key option
 }.
 
 (** A CPA adversary against the KEM is an algorithm: **)
@@ -33,61 +38,66 @@ module type KEM_CPA_Adv = {
   proc distinguish(pk : pkey, k : key, c : kct): bool
 }.
 
-(** And we define the advantage of a CPA adversary A against a KEM E
-    as
-      `|   Pr[KEM_CPA_Exp(E, A).run(false) @ &m: res]
-         - Pr[KEM_CPA_Exp(E, A).run(true) @ &m: res]  |
-    where KEM_CPA_Exp is the experiment:
+(**
+  And we define the advantage of a CPA adversary A against a KEM E
+  as
+    `|   Pr[KEM_CPA_Exp(E, A).run(false) @ &m: res]
+       - Pr[KEM_CPA_Exp(E, A).run(true) @ &m: res]  |
+  where KEM_CPA_Exp is the experiment:
 **)
 module KEM_CPA_Exp (E : KEM) (A : KEM_CPA_Adv) = {
   proc run(b : bool) = {
-    var pk, sk, k0, k1, k, c, r;
+    var pk, sk, k0, k1, c, b';
 
     (pk, sk) <@ E.keygen();
-    (k0, c) <@ E.enc(pk);
+    (k0, c) <@ E.encaps(pk);
     k1 <$ dkey;
-    k <- if b then k1 else k0;
-    r <@ A.distinguish(pk, k, c);
-    return r;
+    b' <@ A.distinguish(pk, if b then k1 else k0, c);
+    return b';
   }
 }.
 
-(** A DEM is a pair of algorithms: **)
+(**
+  A DEM is a pair of algorithms:
+  (We force key generation to be sampling from `dkey`.)
+**)
 module type DEM = {
-  (* We force key generation to be sampling in `dkey` *)
+  (* Normally, we put something like `proc keygen() : key` here *)
   proc enc(k : key, m : pt): dct
   proc dec(k : key, c : dct): pt
 }.
 
 (** A passive/eavesdropping DEM adversary is a pair of algorithms: **)
-module type DEM_PAS_Adv = {
+module type DEM_1CPA_Adv = {
   proc choose(): pt * pt
   proc distinguish(c : dct): bool
 }.
 
-(** And we define the advantage of a passive adversary A against a DEM
-    as
-      `|   Pr[DEM_PAS_Exp(E, A).run(false) @ &m: res]
-         - Pr[DEM_PAS_Exp(E, A).run(true) @ &m: res]  |
-    where DEM_PAS_Exp is the experiment:
+(**
+  And we define the advantage of a passive adversary A against a DEM
+  as
+    `|   Pr[DEM_1CPA_Exp(E, A).run(false) @ &m: res]
+       - Pr[DEM_1CPA_Exp(E, A).run(true) @ &m: res]  |
+  where DEM_1CPA_Exp is the experiment:
 **)
-module DEM_PAS_Exp (E : DEM) (A : DEM_PAS_Adv) = {
+module DEM_1CPA_Exp (E : DEM) (A : DEM_1CPA_Adv) = {
   proc run(b : bool) = {
-    var k, m0, m1, c, r;
+    var k, m0, m1, c, b';
 
     k <$ dkey;
     (m0, m1) <@ A.choose();
     c <@ E.enc(k, if b then m1 else m0);
-    r <@ A.distinguish(c);
-    return r;
+    b' <@ A.distinguish(c);
+    return b';
   }
 }.
 
-(** We have defined our assumptions, we can now define our
-    constructive goal.
+(**
+  We have defined our assumptions, we can now define our
+  constructive goal.
 
-    A public key encryption scheme (with structured ciphertexts!) is a
-    triple of algorithms:
+  A public key encryption scheme (with structured ciphertexts!) is a
+  triple of algorithms:
 **)
 module type PKE = {
   proc keygen(): pkey * skey
@@ -101,31 +111,34 @@ module type PKE_CPA_Adv = {
   proc distinguish(c : kct * dct): bool
 }.
 
-(** The advantage of a CPA adversary A against a PKE E is
-      `|   Pr[PKE_CPA_Exp(E, A).run(false) @ &m: res]
-         - Pr[PKE_CPA_Exp(E, A).run(true) @ &m: res]  |
-    where PKE_CPA_Exp is the experiment:
+(**
+  The advantage of a CPA adversary A against a PKE E is
+    `|   Pr[PKE_CPA_Exp(E, A).run(false) @ &m: res]
+       - Pr[PKE_CPA_Exp(E, A).run(true) @ &m: res]  |
+  where PKE_CPA_Exp is the experiment:
 **)
 module PKE_CPA_Exp (E : PKE) (A : PKE_CPA_Adv) = {
   proc run(b : bool) = {
-    var pk, sk, c, r, m0, m1;
+    var pk, sk, c, b', m0, m1;
 
     (pk, sk) <@ E.keygen();
     (m0, m1) <@ A.choose(pk);
     c <@ E.enc(pk, if b then m1 else m0);
-    r <@ A.distinguish(c);
-    return r;
+    b' <@ A.distinguish(c);
+    return b';
   }
 }.
 
-(* (* Note: instead of defining a specialised notion of PKE with
-      structured ciphertexts, we could have obtained very similar
-      definitions by _instantiating_ a library definition.
+(*
+(*
+  Note: instead of defining a specialized notion of PKE with
+  structured ciphertexts, we could have obtained very similar
+  definitions by _instantiating_ a library definition.
 
-      However, note that the humongous variety of ways in which CPA
-      security for PKEs can be expressed makes developing such a
-      library a tricky proposition.
-   *)
+  However, note that the humongous variety of ways in which CPA
+  security for PKEs can be expressed makes developing such a
+  library a tricky proposition.
+*)
 require PKE.
 clone PKE as KEM_Based_PKE with
   type pkey <= pkey,
@@ -141,11 +154,11 @@ module KEMDEM (E_kem : KEM) (E_s : DEM): PKE = {
   proc keygen = E_kem.keygen
 
   proc enc(pk : pkey, m : pt): kct * dct = {
-    var k, kc, c;
+    var k, kc, dc;
 
-    (k, kc) <@ E_kem.enc(pk);
-    c <@ E_s.enc(k, m);
-    return (kc, c);
+    (k, kc) <@ E_kem.encaps(pk);
+    dc <@ E_s.enc(k, m);
+    return (kc, dc);
   }
 
   proc dec(sk : skey, c : kct * dct): pt option = {
@@ -153,7 +166,7 @@ module KEMDEM (E_kem : KEM) (E_s : DEM): PKE = {
 
     (kc, dc) <- c;
     r <- None;
-    k <@ E_kem.dec(sk, kc);
+    k <@ E_kem.decaps(sk, kc);
     if (k <> None) {
       m <@ E_s.dec(oget k, dc);
       r <- Some m;
@@ -163,32 +176,33 @@ module KEMDEM (E_kem : KEM) (E_s : DEM): PKE = {
 }.
 
 
-(*** And we prove its security: there exist reductions B_kem_0(E_s),
-       B_kem_1(E_s) and B_s(E_kem) such that ...
-***)
-module B_kem_0 (E_s : DEM) (A : PKE_CPA_Adv) = {
-  proc distinguish(pk : pkey, k : key, c: kct) = {
-    var m0, m1, c', r;
+(**
+  And we prove its security: there exist reductions B_kem_0(E_s),
+  B_kem_1(E_s) and B_s(E_kem) such that ...
+**)
+module B_kem_0 (E_s : DEM) (A : PKE_CPA_Adv) : KEM_CPA_Adv = {
+  proc distinguish(pk : pkey, k : key, kc: kct) = {
+    var m0, m1, dc, b';
 
     (m0, m1) <@ A.choose(pk);
-    c' <@ E_s.enc(k, m0);
-    r <@ A.distinguish(c, c');
-    return r;
+    dc <@ E_s.enc(k, m0);
+    b' <@ A.distinguish((kc, dc));
+    return b';
   }
 }.
 
-module B_kem_1 (E_s : DEM) (A : PKE_CPA_Adv) = {
-  proc distinguish(pk : pkey, k : key, c: kct) = {
-    var m0, m1, c', r;
+module B_kem_1 (E_s : DEM) (A : PKE_CPA_Adv) : KEM_CPA_Adv = {
+  proc distinguish(pk : pkey, k : key, kc: kct) = {
+    var m0, m1, dc, b';
 
     (m0, m1) <@ A.choose(pk);
-    c' <@ E_s.enc(k, m1);
-    r <@ A.distinguish(c, c');
-    return r;
+    dc <@ E_s.enc(k, m1);
+    b' <@ A.distinguish((kc, dc));
+    return b';
   }
 }.
 
-module B_s (E_kem : KEM) (A : PKE_CPA_Adv) = {
+module B_s (E_kem : KEM) (A : PKE_CPA_Adv) : DEM_1CPA_Adv = {
   var pk : pkey
 
   proc choose() = {
@@ -199,58 +213,60 @@ module B_s (E_kem : KEM) (A : PKE_CPA_Adv) = {
     return (m0, m1);
   }
 
-  proc distinguish(c : dct) = {
-    var k0, kc, r;
+  proc distinguish(dc : dct) = {
+    var k0, kc, b';
 
-    (k0, kc) <@ E_kem.enc(pk);
-    r <@ A.distinguish(kc, c);
-    return r;
+    (k0, kc) <@ E_kem.encaps(pk);
+    b' <@ A.distinguish((kc, dc));
+    return b';
   }
 }.
 
 section.
-(* For every KEM E_kem *)
+(* for every KEM E_kem, ... *)
 declare module E_kem <: KEM { -B_s }.
-(* For every DEM E_s *)
+(* for every DEM E_s, ... *)
 declare module E_s   <: DEM { -B_s, -E_kem }.
-(* and for every CPA adversary against the PKE KEMDEM(E_kem, E_s) *)
+(* and for every CPA adversary against the PKE KEMDEM(E_kem, E_s), ... *)
 declare module A     <: PKE_CPA_Adv { -B_s, -E_kem, -E_s }.
-(* we have
-        Adv^{CPA}_{KEMDEM(E_kem, E_s)}(A)
-     <=   Adv^{CPA}_{E_kem}(B_kem_0(E_s, A))
-        + Adv^{CPA}_{E_kem}(B_kem_1(E_s, A))
-        + Adv^{PAS}_{E_s}(B_s(E_kem, A))
+(*
+  we have
+    Adv^{CPA}_{KEMDEM(E_kem, E_s)}(A)
+ <=   Adv^{CPA}_{E_kem}(B_kem_0(E_s, A))
+    + Adv^{CPA}_{E_kem}(B_kem_1(E_s, A))
+    + Adv^{1CPA}_{E_s}(B_s(E_kem, A))
 *)
 
-(* The pen and paper proof would use an intermediate game Game1, which
-   is roughly the PKE CPA experiment, but where the DEM encryption is
-   carried out using a random key, instead of one obtained from KEM
-   encapsulation.
+(*
+  The pen and paper proof would use an intermediate game Game1, which
+  is roughly the PKE CPA experiment, but where the DEM encryption is
+  carried out using a random key, instead of one obtained from KEM
+  encapsulation.
 
-   It is clearly at distance Adv^{CPA}_{E_kem} from the PKE CPA
-   experiment on KEMDEM with the same parameter b. (Hop1 and Hop3.)
+  It is clearly at distance Adv^{CPA}_{E_kem} from the PKE CPA
+  experiment on KEMDEM with the same parameter b. (Hop1 and Hop3.)
 
-   The distance between Game1 with b = 0 and Game1 with b = 1 is
-   clearly exactly Adv^{PAS}_{E_s}. (Hop2.)
+  The distance between Game1 with b = 0 and Game1 with b = 1 is
+  clearly exactly Adv^{1CPA}_{E_s}. (Hop2.)
 
-   Defining Game1 is unnecessary for the EasyCrypt proof itself, but
-   helps present it in game-based style.
+  Defining Game1 is unnecessary for the EasyCrypt proof itself, but
+  helps present it in game-based style.
 *)
 local module Game1 = {
   proc run(b : bool) = {
-    var pk, sk, m0, m1, k0, k1, kc, c, r;
+    var pk, sk, m0, m1, k0, k1, kc, dc, b';
 
     (pk, sk) <@ E_kem.keygen();
     (m0, m1) <@ A.choose(pk);
-    (k0, kc) <@ E_kem.enc(pk);
+    (k0, kc) <@ E_kem.encaps(pk);
     k1 <$ dkey;
-    c <@ E_s.enc(k1, if b then m1 else m0);
-    r <@ A.distinguish(kc, c);
-    return r;
+    dc <@ E_s.enc(k1, if b then m1 else m0);
+    b' <@ A.distinguish((kc, dc));
+    return b';
   }
 }.
 
-local lemma pke_0_kem_0 &m:
+local lemma EqPr_PKECPA0_KEMCPA0 &m:
     Pr[PKE_CPA_Exp(KEMDEM(E_kem, E_s), A).run(false) @ &m: res]
   = Pr[KEM_CPA_Exp(E_kem, B_kem_0(E_s, A)).run(false) @ &m: res].
 proof.
@@ -260,18 +276,19 @@ proof.
 byequiv=> //; proc.
 (* We inline the reduction to make the PKE adversary appear on the
    right *)
-inline {2} ^r<@.
+inline {2} 4.
 wp; call (: true). (* if the adversary runs with similar views of the
                       system (state of A, inputs), then they must end
                       with similar views of the system (output) *)
 (* We inline the KEM/DEM's encryption to make encapsulation and DEM
    encryption appear *)
-inline {1} ^c<@.
+inline {1} 3.
 wp; call (: true). (* same on DEM encryption-it's abstract! treated
                       the same as an adversary in our logic *)
 (* We need to align the KEM encapsulation calls and adversary runs;
    fortunately, we know they are independent. *)
-swap {1} ^pk0<- -1. swap {1} -1 -2.
+swap {1} 3 -1.
+swap {1} -1 -2.
 (* We then have a sequence of equivalent calls *)
 wp; call (: true).
 (* interrupted by a one-sided random sampling-a key we do not use *)
@@ -281,14 +298,15 @@ wp; call (: true).
 by auto.
 qed.
 
-local lemma kem_1_game1_0 &m:
+local lemma EqPr_KEMCPA1_Game10 &m:
     Pr[KEM_CPA_Exp(E_kem, B_kem_0(E_s, A)).run(true) @ &m: res]
   = Pr[Game1.run(false) @ &m: res].
 proof.
 (* Once we know how to do the proof, we can automate more of it *)
 byequiv=> //; proc.
-inline {1} ^r<@.
-swap {1} ^pk0<- -3. swap {1} ^c0<- & +1 @^pk0<- & +1.
+inline {1} 4.
+swap {1} 4 -2.
+swap {1} 7 -4.
 sim.
 call (: true); wp.
 conseq (: ={k1, k0, pk, sk, m1, m0, glob E_s, glob A}
@@ -296,48 +314,50 @@ conseq (: ={k1, k0, pk, sk, m1, m0, glob E_s, glob A}
 by sim.
 qed.
 
-local lemma Hop1 &m:
+local lemma GameHop1 &m:
   `| Pr[PKE_CPA_Exp(KEMDEM(E_kem, E_s), A).run(false) @ &m: res]
    - Pr[Game1.run(false) @ &m: res] |
  = `| Pr[KEM_CPA_Exp(E_kem, B_kem_0(E_s, A)).run(false) @ &m: res]
     - Pr[KEM_CPA_Exp(E_kem, B_kem_0(E_s, A)).run(true) @ &m: res] |.
-proof. by rewrite (pke_0_kem_0 &m) -(kem_1_game1_0 &m). qed.
+proof. by rewrite (EqPr_PKECPA0_KEMCPA0 &m) -(EqPr_KEMCPA1_Game10 &m). qed.
 
-local lemma Hop2 &m:
+local lemma GameHop2 &m:
   `| Pr[Game1.run(false) @ &m: res]
    - Pr[Game1.run(true) @ &m: res] |
-  = `| Pr[DEM_PAS_Exp(E_s, B_s(E_kem, A)).run(false) @ &m: res]
-     - Pr[DEM_PAS_Exp(E_s, B_s(E_kem, A)).run(true) @ &m: res] |.
+  = `| Pr[DEM_1CPA_Exp(E_s, B_s(E_kem, A)).run(false) @ &m: res]
+     - Pr[DEM_1CPA_Exp(E_s, B_s(E_kem, A)).run(true) @ &m: res] |.
 proof.
 (* With enough faith, one can shortcut named lemmas *)
 have ->: Pr[Game1.run(false) @ &m: res]
-       = Pr[DEM_PAS_Exp(E_s, B_s(E_kem, A)).run(false) @ &m: res].
+       = Pr[DEM_1CPA_Exp(E_s, B_s(E_kem, A)).run(false) @ &m: res].
 + byequiv=> //; proc.
-  inline {2} ^r<@.
-  swap {2} ^c0<- & +1 -2. swap {2} ^k<$ 2.
+  inline {2} 4.
+  swap {2} 5 -2.
+  swap {2} 1 2.
   inline {2} 1.
   by sim.
 have -> //: Pr[Game1.run(true) @ &m: res]
-          = Pr[DEM_PAS_Exp(E_s, B_s(E_kem, A)).run(true) @ &m: res].
+          = Pr[DEM_1CPA_Exp(E_s, B_s(E_kem, A)).run(true) @ &m: res].
 byequiv=> //; proc.
-swap {2} ^k<$ 1.
-inline {2} ^r<@.
-swap {2} ^c0<- & +1 -3.
+swap {2} 1 1.
+inline {2} 4.
+swap {2} 5 -3.
 inline {2} 1.
 by sim.
 qed.
 
-local lemma Hop3 &m:
-  `| Pr[PKE_CPA_Exp(KEMDEM(E_kem, E_s), A).run(true) @ &m: res]
-   - Pr[Game1.run(true) @ &m: res] |
- = `| Pr[KEM_CPA_Exp(E_kem, B_kem_1(E_s, A)).run(true) @ &m: res]
-    - Pr[KEM_CPA_Exp(E_kem, B_kem_1(E_s, A)).run(false) @ &m: res] |.
+local lemma GameHop3 &m:
+  `| Pr[Game1.run(true) @ &m: res]
+     - Pr[PKE_CPA_Exp(KEMDEM(E_kem, E_s), A).run(true) @ &m: res] |
+ = `| Pr[KEM_CPA_Exp(E_kem, B_kem_1(E_s, A)).run(false) @ &m: res]
+    - Pr[KEM_CPA_Exp(E_kem, B_kem_1(E_s, A)).run(true) @ &m: res] |.
 proof.
 have ->: Pr[PKE_CPA_Exp(KEMDEM(E_kem, E_s), A).run(true) @ &m: res]
        = Pr[KEM_CPA_Exp(E_kem, B_kem_1(E_s, A)).run(false) @ &m: res].
 + byequiv=> //; proc.
   inline *.
-  swap {1} ^pk0<- -1. swap {1} 5 -2.
+  swap {1} 3 -1.
+  swap {1} 5 -2.
   wp; call (: true).
   wp; call (: true).
   wp; call (: true).
@@ -347,7 +367,8 @@ have -> /#: Pr[Game1.run(true) @ &m: res]
           = Pr[KEM_CPA_Exp(E_kem, B_kem_1(E_s, A)).run(true) @ &m: res].
 byequiv=> //; proc.
 inline *.
-swap {2} ^pk0<- -3. swap {2} 8 -5.
+swap {2} 4 -2.
+swap {2} 7 -4.
 sim.
 wp; call (: true).
 wp; rnd.
@@ -357,17 +378,17 @@ by wp; call (: true).
 qed.
 
 (* We can finally conclude! *)
-lemma security_of_kem_dem &m:
+lemma KEMDEM_PKECPA_Security &m:
   `| Pr[PKE_CPA_Exp(KEMDEM(E_kem, E_s), A).run(false) @ &m: res]
    - Pr[PKE_CPA_Exp(KEMDEM(E_kem, E_s), A).run(true) @ &m: res]|
   <= `| Pr[KEM_CPA_Exp(E_kem, B_kem_0(E_s, A)).run(false) @ &m: res]
       - Pr[KEM_CPA_Exp(E_kem, B_kem_0(E_s, A)).run(true) @ &m: res] |
    + `| Pr[KEM_CPA_Exp(E_kem, B_kem_1(E_s, A)).run(false) @ &m: res]
       - Pr[KEM_CPA_Exp(E_kem, B_kem_1(E_s, A)).run(true) @ &m: res] |
-   + `| Pr[DEM_PAS_Exp(E_s, B_s(E_kem, A)).run(false) @ &m: res]
-      - Pr[DEM_PAS_Exp(E_s, B_s(E_kem, A)).run(true) @ &m: res] |.
-proof. smt(Hop1 Hop2 Hop3). qed.
+   + `| Pr[DEM_1CPA_Exp(E_s, B_s(E_kem, A)).run(false) @ &m: res]
+      - Pr[DEM_1CPA_Exp(E_s, B_s(E_kem, A)).run(true) @ &m: res] |.
+proof. smt(GameHop1 GameHop2 GameHop3). qed.
 
 end section.
 
-print security_of_kem_dem.
+print KEMDEM_PKECPA_Security.
